ex/FailureEx.thy
@@ -3,6 +3,14 @@ theory FailureEx
 begin
 
 (* TODO: move *)
+
+lemma non_dependent_all_concl_extract:
+  \<open>p x \<Longrightarrow> (\<forall>x. p x \<longrightarrow> q \<and> r x) \<longleftrightarrow> (\<forall>x. p x \<longrightarrow> r x) \<and> q\<close>
+  \<open>p x \<Longrightarrow> (\<forall>x. p x \<longrightarrow> r x \<and> q) \<longleftrightarrow> (\<forall>x. p x \<longrightarrow> r x) \<and> q\<close>
+  by blast+
+  
+
+
 lemma comp_inf_distrib:
   \<open>(a \<sqinter> b) \<circ> f = (a \<circ> f) \<sqinter> (b \<circ> f)\<close>
   by force
@@ -15,15 +23,64 @@ lemma option_ex_split:
   \<open>(case mx of Some x \<Rightarrow> p x | None \<Rightarrow> q) \<longleftrightarrow> (\<exists>x. mx = Some x \<and> p x) \<or> mx = None \<and> q\<close>
   by (metis case_option_disj_iff)
 
-(* TODO: move *)
-\<comment> \<open> A 'local' predicate that may depend on the shared state. \<close>
-abbreviation(input) local_pred_with_shared
-  :: \<open>('b \<Rightarrow> 'a \<Rightarrow> bool) \<Rightarrow> ('a \<times> 'b \<Rightarrow> bool)\<close> (\<open>\<L>\<^sub>S\<close>)
-  where
-    \<open>\<L>\<^sub>S p \<equiv> \<lambda>(ls, ss). p ss ls\<close>
+lemma pred_times_le_iff:
+  \<open>p \<times>\<^sub>P q \<le> p' \<times>\<^sub>P q' \<longleftrightarrow> p \<le> p' \<and> q \<le> q' \<or> p \<le> \<bottom> \<or> q \<le> \<bottom>\<close>
+  by (force simp add: pred_times_def le_fun_def)
 
-definition (in pre_perm_alg)
-  \<open>all_disjoint_perms \<equiv> {\<pi>::'a. \<forall>\<pi>'. \<not> \<pi> ## \<pi>'}\<close>
+lemma pred_times_le_iff2:
+  \<open>p \<times>\<^sub>P q \<le> p' \<times>\<^sub>P q' \<longleftrightarrow> p \<le> p' \<and> q \<le> q' \<or> (\<nexists>x. p x) \<or> (\<nexists>x. q x)\<close>
+  by (force simp add: pred_times_def le_fun_def)
+
+lemma eqpred_le_iff[simp]:
+  \<open>(=) x \<le> (=) y \<longleftrightarrow> x = y\<close>
+  by force
+
+lemma eqpred_never_empty[simp]:
+  \<open>(=) x \<le> \<bottom> \<longleftrightarrow> False\<close>
+  by force
+
+lemma (in order_bot) disj_leq_bot_iff[simp]:
+  \<open>a \<le> \<bottom> \<or> a \<le> b \<longleftrightarrow> a \<le> b\<close>
+  \<open>a \<le> b \<or> a \<le> \<bottom> \<longleftrightarrow> a \<le> b\<close>
+  by (metis bot.extremum order_eq_iff)+
+
+
+definition capture_fst (\<open>\<lceil> _ \<rceil>\<^sub>1\<close> [0] 999) where
+  \<open>\<lceil> f \<rceil>\<^sub>1 \<equiv> \<lambda>(a,b). f a (a,b)\<close>
+
+definition capture_snd (\<open>\<lceil> _ \<rceil>\<^sub>2\<close> [0] 999) where
+  \<open>\<lceil> f \<rceil>\<^sub>2 \<equiv> \<lambda>(a,b). f b (a,b)\<close>
+
+lemma capture_fst_apply[simp]:
+  \<open>capture_fst f (a,b) = f a (a,b)\<close>
+  by (simp add: capture_fst_def)
+
+lemma capture_snd_apply[simp]:
+  \<open>capture_snd f (a,b) = f b (a,b)\<close>
+  by (simp add: capture_snd_def)
+
+lemma capture_fst_unused[simp]:
+  \<open>\<lceil> \<lambda>s. f \<rceil>\<^sub>1 = f\<close>
+  by (simp add: capture_fst_def)
+
+lemma capture_snd_unused[simp]:
+  \<open>\<lceil> \<lambda>s. f \<rceil>\<^sub>2 = f\<close>
+  \<open>\<lceil> \<lambda>s. f \<sqinter> g s \<rceil>\<^sub>2 = f \<sqinter> \<lceil> \<lambda>s. g s \<rceil>\<^sub>2\<close>
+  \<open>\<lceil> \<lambda>s. g s \<sqinter> f \<rceil>\<^sub>2 = \<lceil> \<lambda>s. g s \<rceil>\<^sub>2 \<sqinter> f\<close>
+  \<open>\<lceil> \<lambda>s. f \<squnion> g s \<rceil>\<^sub>2 = f \<squnion> \<lceil> \<lambda>s. g s \<rceil>\<^sub>2\<close>
+  \<open>\<lceil> \<lambda>s. g s \<squnion> f \<rceil>\<^sub>2 = \<lceil> \<lambda>s. g s \<rceil>\<^sub>2 \<squnion> f\<close>
+  by (force simp add: capture_snd_def)+
+
+lemma capture_snd_idem[simp]:
+  \<open>\<lceil> \<lambda>sa. \<lceil> \<lambda>sb. f sa sb \<rceil>\<^sub>2 \<rceil>\<^sub>2 = \<lceil> \<lambda>s. f s s \<rceil>\<^sub>2\<close>
+  by (simp add: capture_snd_def)
+
+notation(input) capture_snd (\<open>\<lceil> _ \<rceil>\<^sub>\<S>\<close> [0] 999)
+
+
+abbreviation (in pre_perm_alg)
+  \<open>all_disjoint_res \<equiv> \<lambda>a::'a. \<forall>b. \<not> a ## b\<close>
+
 
 section \<open> Helper Lemmas \<close>
 
@@ -33,19 +90,30 @@ lemma heap_upd_eq_iff:
   \<open>ha(x \<mapsto>  va) = hb(x \<mapsto>  vb) \<longleftrightarrow> (\<forall>y. y \<noteq> x \<longrightarrow> ha y = hb y) \<and> va = vb\<close>
   by (force simp add: fun_eq_iff)
 
-lemma not_dom_then_singleton_plus_heap_eq[simp]:
-  \<open>h x = None \<Longrightarrow> [x \<mapsto> v] + h = h(x \<mapsto> v)\<close>
-  by (simp add: fun_eq_iff)
-
 lemma map_empty_disjoint[simp]:
   \<open>Map.empty ## mb\<close>
   \<open>ma ## Map.empty\<close>
   by (simp add: disjoint_fun_def)+
 
+lemma map_upd_disjoint[simp]:
+  \<open>ma x = None \<Longrightarrow> ma(x := va) ## mb \<longleftrightarrow> va ## mb x \<and> ma ## mb\<close>
+  \<open>mb x = None \<Longrightarrow> ma ## mb(x := vb) \<longleftrightarrow> ma x ## vb \<and> ma ## mb\<close>
+   by (clarsimp simp add: disjoint_fun_def disjoint_option_def all_conj_distrib
+      split: option.splits, fastforce)+
+
 lemma map_empty_plus[simp]:
   \<open>Map.empty + mb = mb\<close>
   \<open>ma + Map.empty = ma\<close>
   by (simp add: fun_eq_iff)+
+
+lemma not_dom_then_singleton_plus_heap_eq[simp]:
+  \<open>h x = None \<Longrightarrow> [x \<mapsto> v] + h = h(x \<mapsto> v)\<close>
+  by (simp add: fun_eq_iff)
+
+lemma map_upd_None_over_plus_eq[simp]:
+  \<open>mb x = None \<Longrightarrow> (ma + mb)(x := None) = (ma(x := None) + mb)\<close>
+  \<open>ma x = None \<Longrightarrow> (ma + mb)(x := None) = (ma + mb(x := None))\<close>
+  by fastforce+
 
 lemma singleton_plus_heap_eq_iff:
   \<open>[x \<mapsto> va] + h = [x \<mapsto> vb] + h \<longleftrightarrow> Some va + h x = Some vb + h x\<close>
@@ -54,6 +122,15 @@ lemma singleton_plus_heap_eq_iff:
 lemma heap_upd_eq_singleton_plus_heap_iff:
   \<open>hx(x \<mapsto>  va) = [x \<mapsto> vb] + hy \<longleftrightarrow> (\<forall>y. y \<noteq> x \<longrightarrow> hx y = hy y) \<and> Some vb + hy x = Some va\<close>
   by (force simp add: plus_fun_def plus_option_def fun_eq_iff split: option.splits if_splits)
+
+
+subsubsection \<open> Value at Location \<close>
+
+definition val_at :: \<open>'a \<Rightarrow> ('v \<Rightarrow> bool) \<Rightarrow> ('a \<Rightarrow> 'v) \<Rightarrow> bool\<close> (\<open>\<^bold>@\<close>) where
+  \<open>\<^bold>@ x p \<equiv> \<lambda>f. p (f x)\<close>
+
+definition val_at_heap :: \<open>'a \<Rightarrow> ('v \<Rightarrow> bool) \<Rightarrow> ('a \<rightharpoonup> 'v) \<Rightarrow> bool\<close> (\<open>\<^bold>@\<^sub>\<H>\<close>) where
+  \<open>\<^bold>@\<^sub>\<H> pt p \<equiv> \<lambda>h. \<forall>v. h pt = Some v \<longrightarrow> p v\<close>
 
 
 subsection \<open> Tuple rearrangement \<close>
@@ -118,6 +195,18 @@ lemma comp_ppABC_to_ppACB_mono[intro]:
   \<open>pa \<le> pb \<Longrightarrow> pa \<circ> ppABC_to_ppACB \<le> pb \<circ> ppABC_to_ppACB\<close>
   by (clarsimp simp add: le_fun_def)
 
+lemma wssa_comp_ppABC_to_ppACB_distrib:
+  \<open>wssa R (((p \<times>\<^sub>P q) \<circ> ppABC_to_ppACB)) = ((wssa R p \<times>\<^sub>P q) \<circ> ppABC_to_ppACB)\<close>
+  by (force simp add: fun_eq_iff wlp_def)
+
+lemma sswa_comp_ppABC_to_ppACB_distrib:
+  \<open>sswa R (((p \<times>\<^sub>P q) \<circ> ppABC_to_ppACB)) = ((sswa R p \<times>\<^sub>P q) \<circ> ppABC_to_ppACB)\<close>
+  by (force simp add: fun_eq_iff sp_def)
+
+lemma comp_ppABC_to_ppACB_comp_le_ppABC_to_ppACB_iff[simp]:
+  \<open>(p \<circ> ppABC_to_ppACB) \<le> (q \<circ> ppABC_to_ppACB) \<longleftrightarrow> p \<le> q\<close>
+  by (force simp add: le_fun_def)
+
 
 subsection \<open> Failure \<close>
 
@@ -129,9 +218,19 @@ abbreviation
 abbreviation
   \<open>failure_pred p \<equiv> (p \<times>\<^sub>P (=) Failed) \<circ> ppABC_to_ppACB\<close>
 
+(*
 lemma nofailure_pred_strong_mono[simp]:
   \<open>nofailure_pred p \<le> nofailure_pred q \<longleftrightarrow> p \<le> q\<close>
   by (simp add: le_fun_def)
+
+lemma nofailure_impl_failure_iff[simp]:
+  \<open>nofailure_pred p \<le> failure_pred q \<longleftrightarrow> p \<le> \<bottom>\<close>
+  by (simp add: le_fun_def)
+
+lemma failure_impl_nofailure_iff[simp]:
+  \<open>failure_pred p \<le> nofailure_pred q \<longleftrightarrow> p \<le> \<bottom>\<close>
+  by (simp add: le_fun_def)
+*)
 
 \<comment> \<open> These two only work because the fail_st resources are duplicable, i.e. \<open>a + a = a\<close>. \<close>
 lemma nofailure_pred_sepconj_conj_distrib:
@@ -145,13 +244,38 @@ lemma failure_pred_sepconj_conj_distrib:
   by (force simp add: fun_eq_iff sepconj_conj_def)
 
 
-abbreviation failure_rgsat_pretty
+subsection \<open> Execution with failure \<close>
+
+\<comment> \<open>
+  A fairly standard result.
+  Execution under failure avoidance can be broken into execution where the failure does not happen,
+  and an assurance that the execution can't lead to failure.
+\<close>
+lemma sp_nofailure_pred_in_out_iff:
+  fixes ra :: \<open>('a \<times> fail_st) \<times> 's \<Rightarrow> _ \<Rightarrow> bool\<close>
+  shows
+  \<open>sp ra (nofailure_pred p) \<le> nofailure_pred q \<longleftrightarrow>
+    sp (ra \<circ>\<^sub>2 (\<lambda>(x, y). ((x, Running), y))) p \<le> q \<and>
+    sp ra (nofailure_pred p) \<le> nofailure_pred \<top>\<close>
+  by (force simp add: sp_def le_fun_def)
+
+
+subsection \<open> Pretty RGSat failure judgmeent \<close>
+
+abbreviation fl_rgsat_pretty
   (\<open>_, _, _, _, _ \<turnstile>\<^sub>f { _ } _ { _ }\<close> [55, 0, 0, 0, 0, 55, 55, 55] 56) where
   \<open>R, G, I, F, T \<turnstile>\<^sub>f { p } c { q } \<equiv>
     rgsat c R G
       (nofailure_pred p) (nofailure_pred q)
       (nofailure_pred I) (nofailure_pred F)
       T\<close>
+
+lemmas fl_rgsat_weaken =
+  rgsat_weaken[where
+    p'=\<open>nofailure_pred p'\<close> and q'=\<open>nofailure_pred q'\<close> and
+    I'=\<open>nofailure_pred I'\<close> and F'=\<open>nofailure_pred F'\<close> and
+    p=\<open>nofailure_pred p\<close> and q=\<open>nofailure_pred q\<close> and
+    I=\<open>nofailure_pred I\<close> and F=\<open>nofailure_pred F\<close> for p q I F p' q' I' F', simplified]
 
 
 section \<open> Assert \<close>
@@ -174,27 +298,29 @@ lemmas Assert_def = assert_rel_def
 
 lemma rgsat_assert:
   assumes
-    \<open>p \<^emph>\<and> F \<le> pa\<close>
-    \<open>rel_image snd (rel_liftL (p \<^emph>\<and> F) \<sqinter> (=)) \<le> G\<close>
-    \<open>sswa R p \<le> I\<close>
+    \<open>wssa R p \<^emph>\<and> F \<le> pa\<close>
+    \<open>rel_image snd (rel_liftL (wssa R p \<^emph>\<and> F) \<sqinter> (=)) \<le> G\<close>
+    \<open>wssa R p \<le> I\<close>
     \<open>T RGSepAtom\<close>
   shows
-    \<open>R, G, I, F, T \<turnstile>\<^sub>f { wssa R p } Assert pa { sswa R p }\<close>
+    \<open>R, G, I, F, T \<turnstile>\<^sub>f { wssa R p } Assert pa { wssa R p }\<close>
   using assms
-proof (intro rgsat_atom[where p=\<open>nofailure_pred p\<close> and q=\<open>nofailure_pred p\<close>])
+proof (intro rgsat_atom[where p=\<open>nofailure_pred p\<close> and q=\<open>wssa R (nofailure_pred p)\<close>])
   show
     \<open>\<forall>f\<le>nofailure_pred F.
-      sp (assert_rel pa) (nofailure_pred p \<^emph>\<and> f) \<le> nofailure_pred p \<^emph>\<and> any_shared f\<close>
+      sp (assert_rel pa) (wssa R (nofailure_pred p) \<^emph>\<and> f) \<le>
+        wssa R (nofailure_pred p) \<^emph>\<and> any_shared f\<close>
     using assms(1)
     apply (simp add: assert_rel_def all_subpred_pred_times_eq_res_ppABC_to_ppACB_internalise)
-    apply (clarsimp simp add: sp_def sepconj_conj_def)
-    apply blast
+    apply (clarsimp simp add: sp_def sepconj_conj_def le_fun_def wssa_comp_ppABC_to_ppACB_distrib)
+    apply metis
     done
 
-  show \<open>rel_image snd (rel_liftL (nofailure_pred p \<^emph>\<and> nofailure_pred F) \<sqinter> assert_rel pa) \<le> G\<close>
+  show \<open>rel_image snd (rel_liftL (wssa R (nofailure_pred p) \<^emph>\<and> nofailure_pred F) \<sqinter> assert_rel pa) \<le> G\<close>
     using assms(2)
-    by (fastforce simp add: nofailure_pred_sepconj_conj_distrib[symmetric] assert_rel_def)
-qed (clarsimp simp add: wlp_def sp_def le_fun_def)+
+    by (fastforce simp add: assert_rel_def nofailure_pred_sepconj_conj_distrib[symmetric]
+        wssa_comp_ppABC_to_ppACB_distrib)
+qed (simp add: wssa_comp_ppABC_to_ppACB_distrib sswa_comp_ppABC_to_ppACB_distrib pred_times_le_iff)+
 
 lemma frame_expanding_iff:
   \<open>(\<forall>f\<le>F. (p \<sqinter> pa) \<^emph>\<and> f \<le> (p \<^emph>\<and> any_shared f) \<sqinter> pa) \<longleftrightarrow>
@@ -203,14 +329,19 @@ lemma frame_expanding_iff:
 
 lemma rgsat_assert2:
   assumes
-    \<open>(p \<sqinter> pa) \<^emph>\<and> F \<le> pa\<close>
-    \<open>rel_image snd (rel_liftL ((p \<sqinter> pa) \<^emph>\<and> F) \<sqinter> (=)) \<le> G\<close>
-    \<open>sswa R (p \<sqinter> pa) \<le> I\<close>
+    \<open>wssa R (p \<sqinter> pa) \<^emph>\<and> F \<le> pa\<close>
+    \<open>rel_image snd (rel_liftL (wssa R (p \<sqinter> pa) \<^emph>\<and> F) \<sqinter> (=)) \<le> G\<close>
+    \<open>wssa R (p \<sqinter> pa) \<le> I\<close>
     \<open>T RGSepAtom\<close>
   shows
-    \<open>R, G, I, F, T \<turnstile>\<^sub>f { wssa R (p \<sqinter> pa) } Assert pa { sswa R (p \<sqinter> pa) }\<close>
+    \<open>R, G, I, F, T \<turnstile>\<^sub>f { wssa R (p \<sqinter> pa) } Assert pa { wssa R (p \<sqinter> pa) }\<close>
   using assms
-  by (blast intro: rgsat_assert)
+  by (intro rgsat_assert) simp+
+
+\<comment> \<open> slightly weaker than the full condition, but much more direct \<close>
+lemma guard_frame_expanding_then_assert_framecond:
+  \<open>wssa R pa \<^emph>\<and> F \<le> pa \<Longrightarrow> wssa R (p \<sqinter> pa) \<^emph>\<and> F \<le> pa\<close>
+  by (meson inf_le2 order_trans sepconj_conj_monoL wlp_pred_mono)
 
 lemma opstep_assert_iff[simp]:
   defines \<open>local \<equiv> fst \<circ> fst\<close>
@@ -231,42 +362,55 @@ lemma opstep_assert_iff[simp]:
 section \<open> Heap Predicates \<close>
 
 definition points_to :: \<open>'a \<Rightarrow> 'b \<Rightarrow> ('a \<rightharpoonup> 'b) \<Rightarrow> bool\<close> (infix \<open>\<^bold>\<mapsto>\<close> 90) where
-  \<open>p \<^bold>\<mapsto> x \<equiv> \<lambda>h. h p = Some x \<and> (\<forall>p'. p' \<noteq> p \<longrightarrow> h p' = None)\<close>
+  \<open>p \<^bold>\<mapsto> x \<equiv> (=) [p \<mapsto> x]\<close>
 
-definition points_to_upcl :: \<open>'a \<Rightarrow> 'b \<Rightarrow> ('a \<rightharpoonup> 'b) \<Rightarrow> bool\<close> (infix \<open>\<^bold>\<mapsto>\<^sup>\<Up>\<close> 90) where
+definition points_to_dom_upcl :: \<open>'a \<Rightarrow> 'b \<Rightarrow> ('a \<rightharpoonup> 'b) \<Rightarrow> bool\<close> (infix \<open>\<^bold>\<mapsto>\<^sup>\<Up>\<close> 90) where
   \<open>p \<^bold>\<mapsto>\<^sup>\<Up> x \<equiv> \<lambda>h. h p = Some x\<close>
 
-definition points_to_perm
-  :: \<open>'pt \<Rightarrow> 'perm \<Rightarrow> ('s \<Rightarrow> 'v) \<Rightarrow> ('pt \<rightharpoonup> 'v discr \<times> 'perm) \<times> 's \<Rightarrow> bool\<close>
-  (\<open>_ \<^bold>\<mapsto>\<^bsub>_\<^esub> _\<close> [90,0,90] 90)
-  where
-  \<open>pt \<^bold>\<mapsto>\<^bsub>perm\<^esub> e \<equiv> \<lambda>(ls,ss). (=) [pt \<mapsto> (Discr (e ss), perm)] ls\<close>
 
-lemma points_to_upcl_eq:
+lemma points_to_dom_upcl_eq:
   fixes x :: \<open>'a :: perm_alg\<close>
-  assumes maxsep_x: \<open>\<forall>x'. \<not> x ## x'\<close>
+  assumes maximal_res: \<open>\<forall>x'. \<not> x \<prec> x'\<close>
   shows \<open>pt \<^bold>\<mapsto>\<^sup>\<Up> x = \<top> \<^emph> pt \<^bold>\<mapsto> x\<close>
-  unfolding sepconj_def points_to_def points_to_upcl_def
+  unfolding sepconj_def points_to_def points_to_dom_upcl_def
   apply (clarsimp simp add: fun_eq_iff)
   apply (rename_tac h)
   apply (intro iffI)
    apply (rule_tac x=\<open>h(pt := None)\<close> in exI)
    apply (rule_tac x=\<open>[pt \<mapsto> x]\<close> in exI)
    apply force
-  apply (clarsimp simp add: disjoint_option_def split: option.splits)
-  apply (clarsimp simp add: plus_option_iff)
-  apply (metis disjoint_fun_def disjoint_option_iff(1) disjoint_sym_iff maxsep_x)
+  apply (clarsimp simp add: disjoint_option_def plus_option_def all_conj_distrib
+      split: option.splits)
+  apply (cut_tac maximal_res)
+  apply (metis disjoint_fun_def disjoint_option_simps(1) partial_le_plus2
+      resource_order.le_neq_trans)
   done
+
+
+(*
+definition points_to_perm
+  :: \<open>'pt \<Rightarrow> 'perm \<Rightarrow> ('s \<Rightarrow> 'v) \<Rightarrow> ('pt \<rightharpoonup> 'v discr \<times> 'perm) \<times> 's \<Rightarrow> bool\<close>
+  (\<open>_ \<^bold>\<mapsto>\<^bsub>_\<^esub> _\<close> [90,0,90] 90)
+  where
+  \<open>pt \<^bold>\<mapsto>\<^bsub>perm\<^esub> e \<equiv> \<lambda>(ls,ss). (=) [pt \<mapsto> (Discr (e ss), perm)] ls\<close>
+*)
+
 
 definition \<open>maximal_heap \<equiv> \<lambda>h. \<forall>pt. h pt \<noteq> None\<close>
 
 definition
   \<open>heap_avoiding \<rho> v \<pi> \<equiv> - (\<Squnion>x'\<in>Collect ((##) (Discr v, \<pi>)). \<rho> \<^bold>\<mapsto>\<^sup>\<Up> x')\<close>
 
+lemma res_disjoint_to_memcell_le_heap_avoiding:
+  \<open>(#/#) [\<rho> \<mapsto> (Discr v, \<pi>)] \<le> heap_avoiding \<rho> v \<pi>\<close>
+  by (clarsimp simp add: heap_avoiding_def le_fun_def points_to_dom_upcl_def
+      disjoint_fun_def disjoint_option_def split: option.splits)
+
+
 lemma top_write_heap_avoiding_iff_all_disjoint_perm:
   fixes \<pi> :: \<open>'p::pre_perm_alg\<close>
   shows \<open>\<top> \<le> \<L> (heap_avoiding \<rho> v \<pi>) \<longleftrightarrow> (\<forall>\<pi>'. \<not> \<pi> ## \<pi>')\<close>
-  by (force simp add: heap_avoiding_def points_to_upcl_def le_fun_def)
+  by (force simp add: heap_avoiding_def points_to_dom_upcl_def le_fun_def)
 
 
 abbreviation \<open>heap_pred p \<equiv> (p \<times>\<^sub>P \<top>) \<circ> ppABC_to_ppACB\<close>
@@ -277,272 +421,393 @@ section \<open> Heap Commands \<close>
 subsection \<open> Heap Read \<close>
 
 definition heap_read_rel
-  :: \<open>'x \<Rightarrow> 'pt \<Rightarrow> (
-        (('pt \<rightharpoonup> 'v discr \<times> 'perm) \<times> fail_st) \<times> ('x \<Rightarrow> 'v) \<Rightarrow>
-        (('pt \<rightharpoonup> 'v discr \<times> 'perm) \<times> fail_st) \<times> ('x \<Rightarrow> 'v) \<Rightarrow>
-        bool)\<close>
+  :: \<open>('v \<Rightarrow> 'u) \<Rightarrow> 'x \<Rightarrow> 'pt \<Rightarrow>
+        (('pt \<rightharpoonup> 'v) \<times> fail_st) \<times> ('x \<Rightarrow> 'u) \<Rightarrow>
+        (('pt \<rightharpoonup> 'v) \<times> fail_st) \<times> ('x \<Rightarrow> 'u) \<Rightarrow>
+        bool\<close>
   where
-    \<open>heap_read_rel x pt \<equiv>
+    \<open>heap_read_rel f x pt \<equiv>
       \<lambda>((l,fl),s) ((l',fl'),s').
-        (\<exists>v \<pi>. l pt = Some (v, \<pi>) \<and> l' = l \<and> s' = s(x := the_discr v) \<and> fl' = Running) \<or>
+        (\<exists>v. l pt = Some v \<and> l' = l \<and> s' = s(x := f v) \<and> fl' = Running) \<or>
         (l pt = None \<or> fl = Failed) \<and> l' = l \<and> s' = s \<and> fl' = Failed\<close>
 
-abbreviation \<open>HeapRead x pt \<equiv> \<langle> heap_read_rel x pt \<rangle>\<close>
+abbreviation \<open>HeapRead f x pt \<equiv> \<langle> heap_read_rel f x pt \<rangle>\<close>
 lemmas HeapRead_def = heap_read_rel_def
 
 
 lemma rgsat_heap_read:
-  fixes p :: \<open>('x \<Rightarrow> 'v) \<Rightarrow> bool\<close>
-    and x v R \<pi> pt
-  defines \<open>heap_read_guar \<equiv> (\<lambda>s s'. s' = s(x := v))\<close>
-  and \<open>precond \<equiv> pt \<^bold>\<mapsto>\<^bsub>\<pi>\<^esub> (\<lambda>_. v) \<sqinter> wssa R (\<S> (\<lambda>s. p (s(x := v))))\<close>
-  and \<open>postcond \<equiv> pt \<^bold>\<mapsto>\<^bsub>\<pi>\<^esub> (\<lambda>_. v) \<sqinter> sswa R (\<S> p)\<close>
-assumes
-    \<open>heap_read_guar \<le> G\<close>
-    \<open>precond \<le> I\<close>
-    \<open>postcond \<le> I\<close>
+  fixes X :: 'u
+    and p :: \<open>('x \<Rightarrow> 'u) \<Rightarrow> bool\<close>
+    and x :: 'x
+    and e :: \<open>('x \<Rightarrow> 'u) \<Rightarrow> 'v::pre_perm_alg\<close>
+    and R \<pi> pt u2v
+  defines \<open>heap_read_G \<equiv> (\<lambda>s s'. s' = s(x := u2v (e s)))\<close>
+  defines\<open>precond \<equiv> \<lceil> \<lambda>ss. \<L> (pt \<^bold>\<mapsto> e ss) \<rceil>\<^sub>\<S> \<sqinter> \<S> ((\<lambda>ss. p (ss(x := u2v (e ss)))) \<sqinter> \<^bold>@ x ((=) X))\<close>
+  defines \<open>postcond \<equiv> \<lceil> \<lambda>ss. \<L> (pt \<^bold>\<mapsto> e (ss(x := X))) \<rceil>\<^sub>\<S> \<sqinter> \<S> p\<close>
+  defines \<open>frame_post :: (('a \<rightharpoonup> 'v) \<times> ('x \<Rightarrow> 'u) \<Rightarrow> bool) \<equiv>
+    \<lceil>\<lambda>ss. \<L> (\<^bold>@ pt (\<lambda>mvf. \<forall>vf. mvf = Some vf \<longrightarrow>
+                          (p (ss(x := u2v (e ss))) \<longrightarrow> p (ss(x := u2v (e ss + vf)))) )) \<rceil>\<^sub>\<S>\<close>
+  assumes
+    \<open>heap_read_G \<le> G\<close>
+    \<open>wssa R precond \<le> I\<close>
+    \<open>sswa R postcond \<le> I\<close>
     \<open>T RGSepAtom\<close>
+    and frame_cond:
+    \<open>F \<sqinter> (wssa R precond \<midarrow>\<odot>\<^sub>\<and> \<top>) \<le> frame_post\<close>
   shows
-    \<open>R, G, I, F, T \<turnstile>\<^sub>f { precond } HeapRead x pt { postcond }\<close>
+    \<open>R, G, I, F, T \<turnstile>\<^sub>f { wssa R precond } HeapRead u2v x pt { sswa R postcond }\<close>
   using assms
 proof (intro rgsat_atom[where p=\<open>nofailure_pred precond\<close> and q=\<open>nofailure_pred postcond\<close>])
-  show \<open>nofailure_pred precond \<le> wssa R (nofailure_pred precond)\<close>
-    unfolding precond_def
-    by (clarsimp simp add: wlp_def points_to_perm_def, meson rtranclp_trans)
-  then show \<open>sswa R (nofailure_pred precond) \<le> nofailure_pred I\<close>
-    using assms(5)
-    by (meson order_trans subpred_pred_times_eq_res_ppABC_to_ppACB_iff wlp_weaker_iff_sp_stronger)
+  let ?ra = \<open>(\<lambda>(ls, ss) (ls', ss'). ls' = ls \<and> (\<exists>v. ls pt = Some v \<and> ss' = ss(x := u2v v)))\<close>
 
-  show \<open>sswa R (nofailure_pred postcond) \<le> nofailure_pred postcond\<close>
-    unfolding postcond_def
-    by (clarsimp simp add: sp_def points_to_perm_def, meson rtranclp_trans)
-  then show \<open>sswa R (nofailure_pred postcond) \<le> nofailure_pred I\<close>
-    using assms(6)
-    by (meson order_trans subpred_pred_times_eq_res_ppABC_to_ppACB_iff wlp_weaker_iff_sp_stronger)
+  have nofailure_helper:
+    \<open>\<And>f. sp (heap_read_rel u2v x pt) (nofailure_pred (wssa R precond \<^emph>\<and> f)) \<le> nofailure_pred \<top>\<close>
+    apply (clarsimp simp add: heap_read_rel_def sp_def)
+    apply (elim disjE, force)
+    apply (force simp add: precond_def wlp_def val_at_def points_to_def sepconj_conj_def
+        plus_option_iff)
+    done
+  have rel_helper:
+    \<open>(heap_read_rel u2v x pt \<circ>\<^sub>2 (\<lambda>(x, y). ((x, Running), y))) = ?ra\<close>
+    by (force simp add: heap_read_rel_def fun_eq_iff)
 
-  show
-    \<open>\<forall>f\<le>nofailure_pred F. sp (heap_read_rel x pt) (nofailure_pred precond \<^emph>\<and> f) \<le>
+  let ?frame2 = \<open>\<forall>f\<le>F. sp ?ra (wssa R precond \<^emph>\<and> f) \<le> postcond \<^emph>\<and> any_shared f\<close>
+  let ?frame1 =
+    \<open>\<forall>f\<le>nofailure_pred F. sp (heap_read_rel u2v x pt) (wssa R (nofailure_pred precond) \<^emph>\<and> f) \<le>
+      nofailure_pred postcond \<^emph>\<and> any_shared f\<close>
+
+  have \<open>\<top> = (F \<sqinter> (wssa R precond \<midarrow>\<odot>\<^sub>\<and> \<top>) \<le> frame_post)\<close>
+    using frame_cond
+    by simp
+  also have \<open>... = ?frame2\<close>
+    apply (clarsimp simp add: le_fun_def sp_def imp_ex_conjL imp_conjL sepconj_conj_def
+        septract_conj_def)
+    apply (intro iffI impI allI)
+      (* \<Rightarrow> *)
+     apply (rename_tac f lfs v ss ls fs)
+     apply (drule spec2, drule mp, fast)
+     apply (drule spec, drule mp, rule disjoint_sym, assumption, drule mp, assumption)
+     apply (clarsimp simp add: precond_def postcond_def)
+     apply (simp add: wlp_def val_at_def points_to_def frame_post_def
+        plus_option_iff disjoint_option_iff)
+     apply (subgoal_tac \<open>ls pt = Some (e ss) \<and> (\<forall>pt'. pt' \<noteq> pt \<longrightarrow> ls pt' = None)\<close>)
+      prefer 2
+      apply (metis fun_upd_other fun_upd_same rtranclp.rtrancl_refl)
+     apply clarsimp
+     apply (elim disjE conjE exE)
+      (* ls:Some/fs:None *)
+      apply fastforce
+      (* h:Some/f:Some *)
+     apply (rule_tac x=fs in exI)
+     apply (rule conjI, force)
+     apply (rule conjI, force)
+     apply (rule conjI[rotated], force)
+     apply force
+      (* \<Leftarrow> *)
+    apply (rename_tac fs ss ls)
+    apply (drule_tac x=\<open>(=) (fs, ss)\<close> in spec, drule mp, fast)
+    apply (subgoal_tac \<open>ls = [pt \<mapsto> e ss]\<close>)
+     prefer 2
+     apply (fastforce simp add: precond_def wlp_def points_to_def)
+    apply (case_tac \<open>fs pt\<close>)
+      (** \<open>fs pt = None\<close> *)
+     apply (simp add: frame_post_def val_at_def; fail)
+      (** \<open>fs pt = Some ...\<close> *)
+    apply (rename_tac vf)
+    apply (drule_tac x=\<open>ls + fs\<close> and y=\<open>e ss + vf\<close> in spec2, drule mp, force)
+    apply clarsimp
+    apply (drule_tac x=\<open>[pt \<mapsto> e ss]\<close> in spec)
+    apply (simp add: postcond_def frame_post_def)
+    apply (clarsimp simp add: disjoint_sym_iff val_at_def points_to_def fun_eq_iff plus_option_iff
+        if_distrib[of \<open>\<lambda>x. x = _\<close>] if_distrib[of \<open>\<lambda>x. x + _ = _\<close>] if_bool_eq_conj all_conj_distrib
+        eq_commute[of _ \<open>_ pt\<close>])
+    done
+  also have \<open>... = ?frame1\<close>
+    apply (simp add: wssa_comp_ppABC_to_ppACB_distrib)
+    apply (simp add: all_subpred_pred_times_eq_res_ppABC_to_ppACB_internalise
+        nofailure_pred_sepconj_conj_distrib[symmetric]
+        any_shared_pred_times_eq_res_ppABC_to_ppACB_distrib pred_times_le_iff)
+    apply (subst sp_nofailure_pred_in_out_iff)
+    apply (simp add: nofailure_helper rel_helper)
+    done
+  finally show
+    \<open>\<forall>f\<le>nofailure_pred F. sp (heap_read_rel u2v x pt) (wssa R (nofailure_pred precond) \<^emph>\<and> f) \<le>
       nofailure_pred postcond \<^emph>\<and> any_shared f\<close>
     unfolding any_shared_def precond_def postcond_def
-    apply (simp add: all_subpred_pred_times_eq_res_ppABC_to_ppACB_internalise)
-    apply (clarsimp simp add: sp_def points_to_perm_def sepconj_conj_def heap_read_rel_def)
-    apply (clarsimp simp add: plus_option_def split: option.splits)
-     apply (metis (mono_tags) comp_apply not_dom_then_singleton_plus_heap_eq wssa_trivial
-        rtranclp.rtrancl_refl snd_conv)
-    apply (metis (mono_tags) comp_apply rtranclp.rtrancl_refl snd_conv wssa_trivial)
-    done
+    by simp
 
-  show \<open>rel_image snd (rel_liftL (nofailure_pred precond \<^emph>\<and> nofailure_pred F) \<sqinter> heap_read_rel x pt)
-          \<le> G\<close>
-    using assms(4)
-    unfolding heap_read_guar_def precond_def
-    by (force simp add: heap_read_rel_def sepconj_conj_def plus_option_iff points_to_perm_def)
-qed simp+
+  show \<open>rel_image snd (rel_liftL (wssa R (nofailure_pred precond) \<^emph>\<and>
+          nofailure_pred F) \<sqinter> heap_read_rel u2v x pt) \<le> G\<close>
+    using assms(5)
+    unfolding heap_read_G_def precond_def
+    apply (clarsimp simp add: wssa_comp_ppABC_to_ppACB_distrib heap_read_rel_def sepconj_conj_def
+        plus_option_iff ex_disj_distrib conj_disj_distribR wlp_def points_to_def val_at_def)
+    sledgehammer
+    sorry
+qed (simp add: sswa_comp_ppABC_to_ppACB_distrib wssa_comp_ppABC_to_ppACB_distrib pred_times_le_iff)+
 
 
 subsection \<open> Heap Write \<close>
 
-definition heap_write_rel
-  :: \<open>'pt \<Rightarrow> ('s \<Rightarrow> 'v) \<Rightarrow> ((('pt \<rightharpoonup> 'v discr \<times> 'perm) \<times> fail_st) \<times> 's) \<Rightarrow> _ \<Rightarrow> bool\<close>
+definition heap_upd_rel
+  :: \<open>'pt \<Rightarrow> ('a \<Rightarrow> 's \<Rightarrow> 'a) \<Rightarrow> ((('pt \<rightharpoonup> 'a) \<times> fail_st) \<times> 's) \<Rightarrow> _ \<Rightarrow> bool\<close>
   where
-    \<open>heap_write_rel pt e \<equiv>
+    \<open>heap_upd_rel pt e \<equiv>
       \<lambda>((l,fl),s) ((l',fl'),s').
         s' = s \<and> (
-          (\<exists>v perm. l pt = Some (v, perm) \<and> fl = Running \<and> l' = l(pt \<mapsto> (Discr (e s), perm)) \<and> fl' = Running) \<or>
+          (\<exists>v. l pt = Some v \<and> fl = Running \<and> l' = l(pt \<mapsto> e v s) \<and> fl' = Running) \<or>
           (l pt = None \<or> fl = Failed) \<and> l' = l \<and> fl' = Failed)\<close>
 
-abbreviation \<open>HeapWrite pt e \<equiv> \<langle> heap_write_rel pt e \<rangle>\<close>
+abbreviation \<open>HeapUpd pt e \<equiv> \<langle> heap_upd_rel pt e \<rangle>\<close>
 
-
-lemma heap_write_rel_nofailure_rel_eq:
-  \<open>sp (heap_write_rel pt e) (nofailure_pred p) =
-    nofailure_pred (
-      sp
-        (\<lambda>(l,s) (l',s'). s' = s \<and> (\<exists>v perm. l pt = Some (v, perm) \<and> l' = l(pt \<mapsto> (Discr (e s), perm))))
-        p)
-    \<squnion> failure_pred ((\<lambda>(l',s'). l' pt = None) \<sqinter> p)\<close>
-  apply (clarsimp simp add: heap_write_rel_def sp_def fun_eq_iff split: prod.splits)
-  apply (case_tac b, force)
-  apply clarsimp
-  apply (metis (no_types, lifting) ext)
-  done
-
-lemma rgsat_heap_write:
-  fixes e pt p R \<pi> v
-  defines \<open>precond \<equiv> (pt \<^bold>\<mapsto>\<^bsub>\<pi>\<^esub> (\<lambda>_. v)) \<sqinter> wssa R (\<S> p)\<close>
-    and \<open>postcond \<equiv> sswa R (pt \<^bold>\<mapsto>\<^bsub>\<pi>\<^esub> e \<sqinter> \<S> p)\<close>
+lemma rgsat_heap_update:
+  fixes e :: \<open>'s \<Rightarrow> 'v::pre_perm_alg\<close>
+    and e' :: \<open>'v \<Rightarrow> 's \<Rightarrow> 'v\<close>
+    and pt \<pi> p R
+  defines \<open>precond \<equiv> \<lceil> \<lambda>ss. \<L> (pt \<^bold>\<mapsto> e ss) \<rceil>\<^sub>\<S> \<sqinter> \<S> p\<close>
+    and \<open>postcond \<equiv> \<lceil> \<lambda>ss. \<L> (pt \<^bold>\<mapsto> e' (e ss) ss) \<rceil>\<^sub>\<S> \<sqinter> \<S> p\<close>
+    and \<open>frame_post \<equiv>
+          \<lceil> \<lambda>ss. \<L> (\<^bold>@\<^sub>\<H> pt (\<lambda>vf. e' (e ss) ss ## vf \<and> e' (e ss + vf) ss = e' (e ss) ss + vf)) \<rceil>\<^sub>\<S>\<close>
   assumes
-    \<comment> \<open> this is the side condition that constrains permissions to be exclusive \<close>
-    \<open>F \<le> \<L> (heap_avoiding pt v \<pi>)\<close>
+    \<open>F \<sqinter> (wssa R precond \<midarrow>\<odot>\<^sub>\<and> \<top>) \<le> frame_post\<close>
     \<open>(=) \<le> G\<close>
-    \<open>precond \<le> I\<close>
-    \<open>postcond \<le> I\<close>
+    \<open>wssa R precond \<le> I\<close>
+    \<open>sswa R postcond \<le> I\<close>
     \<open>T RGSepAtom\<close>
   shows
-    \<open>R, G, I, F, T \<turnstile>\<^sub>f { precond } HeapWrite pt e { postcond }\<close>
+    \<open>R, G, I, F, T \<turnstile>\<^sub>f { wssa R precond } HeapUpd pt e' { sswa R postcond }\<close>
   using assms
 proof (intro rgsat_atom[where p=\<open>nofailure_pred precond\<close> and q=\<open>nofailure_pred postcond\<close>])
-  show \<open>nofailure_pred precond \<le> wssa R (nofailure_pred precond)\<close>
-    unfolding precond_def
-    by (clarsimp simp add: points_to_perm_def wlp_def, meson rtranclp_trans)
-  then show \<open>sswa R (nofailure_pred precond) \<le> nofailure_pred I\<close>
-    by (meson assms(5) nofailure_pred_strong_mono order_trans wlp_weaker_iff_sp_stronger)
 
-  show \<open>sswa R (nofailure_pred postcond) \<le> nofailure_pred postcond\<close>
-    unfolding postcond_def
-    by (clarsimp simp add: points_to_perm_def sp_def, metis rtranclp_trans)
-  then show \<open>sswa R (nofailure_pred postcond) \<le> nofailure_pred I\<close>
-    using assms(6) by fastforce
+  have helper:
+    \<open>\<And>f. (\<lambda>(l', s'). l' pt = None) \<sqinter> (wssa R precond \<^emph>\<and> f) \<le> \<bottom>\<close>
+    apply (clarsimp simp add: precond_def points_to_def fun_eq_iff sp_def sepconj_conj_def wlp_def
+        plus_option_iff split: prod.splits)
+    apply (metis not_None_eq rtranclp.rtrancl_refl)
+    done
 
-  have failure_helper: \<open>\<And>f. failure_pred ((\<lambda>(l', s'). l' pt = None) \<sqinter> (precond \<^emph>\<and> f)) = \<bottom>\<close>
-    by (clarsimp simp add: fun_eq_iff precond_def points_to_perm_def sepconj_conj_def
-        plus_option_iff, blast)
+  let ?ra = \<open>\<lambda>(l, s) (l', s'). s' = s \<and> (\<exists>v. l pt = Some v \<and> l' = l(pt \<mapsto> e' v s))\<close>
 
-  let ?ra = \<open>(\<lambda>(l, s) (l', s'). s' = s \<and> (\<exists>v perm. l pt = Some (v, perm) \<and> l' = l(pt \<mapsto> (Discr (e s), perm))))\<close>
-  let ?frame2 =
-    \<open>\<forall>f\<le>F. sp ?ra (precond \<^emph>\<and> f) \<le> postcond \<^emph>\<and> any_shared f\<close>
+  let ?frame2 = \<open>\<forall>f\<le>F. sp ?ra (wssa R precond \<^emph>\<and> f) \<le> postcond \<^emph>\<and> any_shared f\<close>
   let ?frame1 =
     \<open>\<forall>f\<le>nofailure_pred F.
-      sp (heap_write_rel pt e) (nofailure_pred precond \<^emph>\<and> f) \<le>
+      sp (heap_upd_rel pt e') (wssa R (nofailure_pred precond) \<^emph>\<and> f) \<le>
         nofailure_pred postcond \<^emph>\<and> any_shared f\<close>
 
-  have \<open>\<top> = ?frame2\<close>
-    using assms(3)
-    unfolding precond_def postcond_def
-    apply (clarsimp simp add: sp_def le_fun_def points_to_perm_def sepconj_conj_def plus_option_iff)
-    apply (elim disjE)
-      (* None case *)
-     apply clarsimp
-     apply (rename_tac s l)
-     apply (rule_tac x=\<open>[pt \<mapsto> (Discr (e s), \<pi>)]\<close> in exI)
-     apply (rule_tac x=l in exI)
-     apply (intro conjI)
-        apply fastforce
-       apply fastforce
+  have helper1: \<open>(heap_upd_rel pt e' \<circ>\<^sub>2 (\<lambda>(x, y). ((x, Running), y))) = ?ra\<close>
+    by (clarsimp simp add: heap_upd_rel_def fun_eq_iff)
+  have helper2:
+    \<open>\<And>f. sp (heap_upd_rel pt e') (nofailure_pred (wssa R precond \<^emph>\<and> f)) \<le> nofailure_pred \<top>\<close>
+    unfolding heap_upd_rel_def precond_def
+    by (force simp add: sepconj_conj_apply sp_def plus_option_iff wlp_def points_to_def)
+
+  have \<open>\<top> = (F \<sqinter> (wssa R precond \<midarrow>\<odot>\<^sub>\<and> \<top>) \<le> frame_post)\<close>
+    using assms(4) by simp
+  also have \<open>(F \<sqinter> (wssa R precond \<midarrow>\<odot>\<^sub>\<and> \<top>) \<le> frame_post) = ?frame2\<close>
+    apply (clarsimp simp add: sp_def le_fun_def sepconj_conj_def)
+    apply (rule iffI)
+      (* \<Rightarrow> *)
+     apply (clarsimp simp add: imp_conjL plus_option_iff)
+     apply (rename_tac f ss v ls fs)
+     apply (drule spec2, drule mp, blast)
+     apply (drule mp, simp add: septract_conj_def, metis disjoint_sym)
+     apply (clarsimp simp add: precond_def postcond_def frame_post_def wlp_def points_to_def
+        disjoint_option_iff)
+     apply (case_tac \<open>ls pt = None\<close>)
+      (** \<open>ls pt = None\<close> *)
+      apply force
+      (** \<open>ls pt = Some ...\<close> *)
+     apply (clarsimp simp add:  plus_option_iff wlp_def)
+     apply (rename_tac v)
+     apply (subgoal_tac \<open>ls pt = Some (e ss) \<and> (\<forall>pt'. pt' \<noteq> pt \<longrightarrow> ls pt' = None)\<close>)
+      prefer 2
       apply fastforce
-     apply fastforce
-      (* Some case, prevented by frame exclusivity *)
-    apply clarsimp
-    apply (rename_tac ss fs v' \<pi>')
-    apply (subgoal_tac \<open>v' = Discr v\<close>)
-     prefer 2
-     apply (simp add: disjoint_fun_def disjoint_option_def split: option.splits)
+     apply (clarsimp simp add: plus_option_def wlp_def disjoint_option_iff split: option.splits)
+      (* as there is only one source of a frame that passes predicate \<open>f\<close>, there is only one
+          frame that will work here. *)
+     apply (rule_tac x=fs in exI)
+     apply (rule conjI, force simp add: val_at_heap_def)
+     apply (elim disjE; simp?)
+      (*** \<open> fs pt = None \<close> *)
+      apply (force simp add: fun_eq_iff)
+      (*** \<open> fs pt = Some ... \<close> *)
+     apply (clarsimp simp add: fun_eq_iff if_bool_eq_disj if_distrib[of \<open>\<lambda>x. x = _\<close>] val_at_heap_def)
      apply metis
-    apply (subgoal_tac \<open>\<pi> ## \<pi>'\<close>)
+      (* \<Leftarrow> *)
+    apply (clarsimp simp add: septract_conj_def imp_ex_conjL imp_conjL)
+    apply (rename_tac fs ss ls)
+    apply (drule_tac x=\<open>(=) (fs, ss)\<close> in spec, drule mp, blast)
+    apply (drule_tac x=ss in spec)
+    apply (drule_tac x=\<open>ls + fs\<close> in spec)
+    apply (subgoal_tac \<open>ls pt = Some (e ss)\<close>)
      prefer 2
+     apply (force simp add: precond_def wlp_def points_to_def)
+    apply (case_tac \<open>fs pt\<close>)
+      (*** \<open> fs pt = None \<close> *)
+     apply (drule_tac x=\<open>e ss\<close> in spec)
+     apply (drule mp, force simp add: precond_def points_to_def)
      apply clarsimp
-     apply (metis disjoint_fun_def disjoint_option_simps(1) disjoint_prod_def fun_upd_same snd_conv)
-    apply (simp add: heap_avoiding_def points_to_upcl_def)
-    apply blast
+     apply (drule spec, drule mp, rule disjoint_sym, assumption)
+     apply (simp add: postcond_def frame_post_def val_at_heap_def; fail)
+      (*** \<open> fs pt = Some ... \<close> *)
+    apply (clarsimp simp add: plus_option_iff imp_conjL)
+    apply (drule spec, drule mp, rule disjoint_sym, assumption)
+    apply clarsimp
+    apply (simp add: precond_def postcond_def frame_post_def val_at_heap_def points_to_def
+        heap_upd_eq_singleton_plus_heap_iff; fail)
     done
   also have \<open>... = ?frame1\<close>
-    by (simp add: all_subpred_pred_times_eq_res_ppABC_to_ppACB_internalise failure_helper
-        nofailure_pred_sepconj_conj_distrib[symmetric] heap_write_rel_nofailure_rel_eq
-        any_shared_pred_times_eq_res_ppABC_to_ppACB_distrib)
+    apply (simp add: wssa_comp_ppABC_to_ppACB_distrib)
+    apply (simp add: all_subpred_pred_times_eq_res_ppABC_to_ppACB_internalise
+        nofailure_pred_sepconj_conj_distrib[symmetric]
+        any_shared_pred_times_eq_res_ppABC_to_ppACB_distrib pred_times_le_iff)
+    apply (subst sp_nofailure_pred_in_out_iff)
+    apply (simp add: helper1 helper2)
+    done
   finally show ?frame1
-    by simp
+    using assms(3)
+    by clarsimp
 
   show
-    \<open>rel_image snd (rel_liftL (nofailure_pred precond \<^emph>\<and> nofailure_pred F) \<sqinter> heap_write_rel pt e) \<le>
-      G\<close>
-    using assms(4)
-    by (clarsimp simp add: heap_write_rel_def nofailure_pred_sepconj_conj_distrib[symmetric]
-        le_fun_def)
-qed simp+
+    \<open>rel_image snd (rel_liftL (wssa R (nofailure_pred precond) \<^emph>\<and> nofailure_pred F) \<sqinter>
+      heap_upd_rel pt e') \<le> G\<close>
+    using assms(5)
+    unfolding precond_def  heap_upd_rel_def
+    by fastforce
+qed (simp add: sswa_comp_ppABC_to_ppACB_distrib wssa_comp_ppABC_to_ppACB_distrib pred_times_le_iff)+
 
 
 subsection \<open> Heap Alloc \<close>
 
 definition heap_alloc_rel
-  :: \<open>('pt \<Rightarrow> 'v) \<Rightarrow>
-        'x \<Rightarrow>
-        (('x \<Rightarrow> 'v) \<Rightarrow> 'v) \<Rightarrow>
-        ((('pt \<rightharpoonup> 'v discr \<times> 'perm::pre_perm_alg) \<times> fail_st) \<times> ('x \<Rightarrow> 'v)) \<Rightarrow> _ \<Rightarrow> bool\<close>
+  :: \<open>('pt \<Rightarrow> 'a::pre_perm_alg) \<Rightarrow> 'x \<Rightarrow> (('x \<Rightarrow> 'a) \<Rightarrow> 'a) \<Rightarrow>
+        ((('pt \<rightharpoonup> 'a) \<times> fail_st) \<times> ('x \<Rightarrow> 'a)) \<Rightarrow> _ \<Rightarrow> bool\<close>
   where
     \<open>heap_alloc_rel Ptr x e \<equiv>
       \<lambda>((l,fl),s) ((l',fl'),s').
-        (\<exists>pt \<pi>. l pt = None \<and> (\<forall>\<pi>'. \<not> \<pi> ## \<pi>') \<and>
-          l' = l(pt \<mapsto> (Discr (e s), \<pi>)) \<and> s' = s(x := Ptr pt) \<and>
+        (\<exists>pt.
+          l pt = None \<and> l' = l(pt \<mapsto> e s) \<and>
+          s' = s(x := Ptr pt) \<and>
           fl = Running \<and> fl' = fl) \<or>
-        (fl = Failed \<or> (\<forall>pt. l pt \<noteq> None) \<or> (\<forall>\<pi>::'perm. \<exists>\<pi>'. \<pi> ## \<pi>')) \<and>
+        (fl = Failed \<or> (\<forall>pt. l pt \<noteq> None)) \<and>
           l' = l \<and> s' = s \<and> fl' = Failed\<close>
 
 abbreviation \<open>HeapAlloc Ptr x e \<equiv> \<langle> heap_alloc_rel Ptr x e \<rangle>\<close>
 
 lemma rgsat_heap_alloc:
-  fixes p pt e R
-  defines \<open>precond \<equiv> \<L> emp \<sqinter> wssa R (\<S> p)\<close>
-    \<comment> \<open> we only obtain \<^emph>\<open>some\<close> totally disjoint permission \<close>
-    and \<open>postcond \<equiv>
-      (\<Squnion>pt. \<Squnion>\<pi>1\<in>all_disjoint_perms. sswa R (pt \<^bold>\<mapsto>\<^bsub>\<pi>1::'perm::pre_perm_alg\<^esub> e \<sqinter> \<S> p))\<close>
+  fixes p pt e R F x X Ptr
+  defines \<open>precond \<equiv> \<L> emp \<sqinter> \<S> (p \<sqinter> \<^bold>@ x ((=) X))\<close>
+  defines \<open>postcond \<equiv> \<Squnion>pt. \<lceil> \<lambda>ss. \<L> (pt \<^bold>\<mapsto> e (ss(x := X))) \<rceil>\<^sub>\<S> \<sqinter> \<S> (\<lambda>ss. p (ss(x := X)) \<and> ss x = Ptr pt)\<close>
   assumes
     \<open>(\<lambda>s s'. \<exists>pt. s' = s(x := Ptr pt)) \<le> G\<close>
-    \<open>precond \<le> I\<close>
-    \<open>postcond \<le> I\<close>
+    \<open>wssa R precond \<le> I\<close>
+    \<open>sswa R postcond \<le> I\<close>
     \<open>T RGSepAtom\<close>
-    and frame_not_maximal_heap: \<open>F \<le> - (\<L> maximal_heap)\<close>
-    and maximal_perm_ex: \<open>\<exists>\<pi>::'perm. \<forall>\<pi>'. \<not> \<pi> ## \<pi>'\<close>
-    and p_alloc_var_irrel: \<open>\<And>ss pt. p (ss(x := Ptr pt)) = p ss\<close>
-    and e_alloc_var_irrel: \<open>\<And>ss ss' pt. e (ss(x := Ptr pt)) = e ss'\<close>
+    and frame_cond: \<open>F \<sqinter> (wssa R precond \<midarrow>\<odot>\<^sub>\<and> \<top>) \<le> - \<L> maximal_heap\<close>
   shows
-    \<open>R, G, I, F, T \<turnstile>\<^sub>f { precond } HeapAlloc Ptr x e { postcond }\<close>
+    \<open>R, G, I, F, T \<turnstile>\<^sub>f { wssa R precond } HeapAlloc Ptr x e { sswa R postcond }\<close>
   using assms
 proof (intro rgsat_atom[where p=\<open>nofailure_pred precond\<close> and q=\<open>nofailure_pred postcond\<close>])
-  show \<open>nofailure_pred precond \<le> wssa R (nofailure_pred precond)\<close>
-    unfolding precond_def
-    by (clarsimp simp add: wlp_def emp_def, meson rtranclp_trans)
-  then show \<open>sswa R (nofailure_pred precond) \<le> nofailure_pred I\<close>
-    using assms(5)
-    by (meson nofailure_pred_strong_mono order.trans wlp_weaker_iff_sp_stronger)
 
-  show \<open>sswa R (nofailure_pred postcond) \<le> nofailure_pred postcond\<close>
-    unfolding postcond_def
-    by (clarsimp simp add: points_to_perm_def sp_def heap_upd_eq_iff, metis rtranclp_trans)
-  then show \<open>sswa R (nofailure_pred postcond) \<le> nofailure_pred I\<close>
-    using assms(6) nofailure_pred_strong_mono by blast
+  let ?ra = \<open>\<lambda>(l, s) (l', s'). 
+              \<exists>pt.
+                l pt = None \<and> l' pt = Some (e s) \<and>
+                (\<forall>pt'. pt' \<noteq> pt \<longrightarrow> l' pt' = l pt') \<and>
+                s' x = Ptr pt \<and>
+                (\<forall>x'. x' \<noteq> x \<longrightarrow> s' x' = s x')\<close>
 
-  show \<open>\<forall>f\<le>nofailure_pred F. sp (heap_alloc_rel Ptr x e) (nofailure_pred precond \<^emph>\<and> f) \<le> nofailure_pred postcond \<^emph>\<and> any_shared f\<close>
-    unfolding precond_def postcond_def
+  have atomrel_helper: \<open>heap_alloc_rel Ptr x e \<circ>\<^sub>2 (\<lambda>(x, y). ((x, Running), y)) = ?ra\<close>
+    by (clarsimp simp add: fun_eq_iff heap_alloc_rel_def all_conj_distrib)
+
+  have
+    \<open>(F \<sqinter> (wssa R precond \<midarrow>\<odot>\<^sub>\<and> \<top>) \<le> - \<L> maximal_heap) =
+      (\<forall>f\<le>F. sp (heap_alloc_rel Ptr x e) (nofailure_pred (wssa R precond \<^emph>\<and> f)) \<le> nofailure_pred \<top>)\<close>
+    apply (clarsimp simp add: sp_def sepconj_conj_apply septract_conj_def le_fun_def
+        imp_conjL imp_ex_conjL)
+    apply (intro iffI allI impI)
+      (* \<Rightarrow> *)
+     apply (rename_tac lsf' fl' ss' ss ls fs)
+     apply (drule spec2, drule mp, blast)
+     apply (drule spec, drule mp, rule disjoint_sym, assumption, drule mp, assumption)
+     apply (clarsimp simp add: heap_alloc_rel_def)
+     apply (elim disjE, fast)
+     apply (clarsimp simp add: plus_option_iff ex_disj_distrib wlp_def emp_def
+        precond_def maximal_heap_def)
+     apply (drule_tac x=pt in spec)
+     apply force
+        (* \<Leftarrow> *)
+    apply clarsimp
+    apply (drule spec, drule mp, fast)
+    apply (clarsimp simp add: heap_alloc_rel_def all_conj_distrib precond_def wlp_def emp_def
+        imp_ex_conjL imp_conjL maximal_heap_def)
+    apply (rename_tac fs ss ls)
+    apply (drule_tac x=fs in spec, drule mp[of \<open>All _\<close>], fast)
+    apply (metis map_empty_disjoint(1) map_empty_plus(1))
+    done
+  then have nofailure_helper:
+    \<open>\<forall>f\<le>F. sp (heap_alloc_rel Ptr x e) (nofailure_pred (wssa R precond \<^emph>\<and> f)) \<le> nofailure_pred \<top>\<close>
+    using frame_cond
+    by simp
+
+  let ?frame2 = \<open>\<forall>f\<le>F. sp ?ra (wssa R precond \<^emph>\<and> f) \<le> postcond \<^emph>\<and> any_shared f\<close>
+  let ?frame1 =
+    \<open>\<forall>f\<le>nofailure_pred F.
+      sp (heap_alloc_rel Ptr x e) (wssa R (nofailure_pred precond) \<^emph>\<and> f) \<le>
+        nofailure_pred postcond \<^emph>\<and> any_shared f\<close>
+
+  have \<open>\<top> = ?frame2\<close>
+    apply clarsimp
+    apply (clarsimp simp add: precond_def postcond_def sp_def emp_def sepconj_conj_def wlp_def
+        points_to_def)
+    apply (rename_tac f lfs' ss' ss pt ls fs)
+    apply (subgoal_tac \<open>ls = Map.empty\<close>)
+     prefer 2
+     apply blast
+    apply clarsimp
+    apply (subgoal_tac \<open>ss'(x := X) = ss\<close>)
+     prefer 2
+     apply (fastforce simp add: val_at_def)
+    apply simp \<comment> \<open> do \<^emph>\<open>not\<close> clarify \<close>
+    apply (thin_tac \<open>ss'(x := X) = ss\<close>)
+    apply (rule_tac x=\<open>[pt \<mapsto> e ss]\<close> in exI)
+    apply (rule_tac x=fs in exI)
+    apply force
+    done
+  also have \<open>?frame2 = ?frame1\<close>
+    apply (simp add: wssa_comp_ppABC_to_ppACB_distrib)
     apply (simp add: all_subpred_pred_times_eq_res_ppABC_to_ppACB_internalise
         nofailure_pred_sepconj_conj_distrib[symmetric]
-        any_shared_pred_times_eq_res_ppABC_to_ppACB_distrib)
-    apply (clarsimp simp add: heap_alloc_rel_def sp_def wlp_def emp_def le_fun_def sepconj_conj_def)
-    apply (rename_tac l fl ls fs ss)
-    apply (elim disjE conjE)
-      apply (clarsimp simp add: points_to_perm_def)
-      apply (simp add: ex_simps[symmetric] del: ex_simps)
-      apply (rule_tac x=\<open>[pt \<mapsto> (Discr (e ss), \<pi>)]\<close> in exI)
-      apply (rule_tac x=fs in exI)
-      apply (rule_tac x=ss in exI)
-      apply (rule_tac x=pt in exI)
-      apply (clarsimp simp add: all_disjoint_perms_def disjoint_fun_def heap_upd_eq_iff)
-      apply (metis e_alloc_var_irrel p_alloc_var_irrel rtranclp.rtrancl_refl)
-      (* contradiction between maximal frame and no maximal frame assumption. *)
-     apply (cut_tac frame_not_maximal_heap)
-     apply (clarsimp simp add: Sup_fun_def sepconj_conj_def ex_simps(1-4)[symmetric]
-        emp_def le_fun_def maximal_heap_def simp del: ex_simps(1-4))
-     apply (metis not_Some_prod_eq)
-      (* contradiction between no maximal perm and maximal_perm_ex assumption. *)
-    apply (cut_tac maximal_perm_ex)
-    apply fast
+        any_shared_pred_times_eq_res_ppABC_to_ppACB_distrib pred_times_le_iff)
+    apply (subst sp_nofailure_pred_in_out_iff)
+    apply (clarsimp simp add: atomrel_helper nofailure_helper)
     done
+  finally show \<open>?frame1\<close>
+    by simp
 
   show
-    \<open>rel_image snd (rel_liftL (nofailure_pred precond \<^emph>\<and> nofailure_pred F) \<sqinter>
+    \<open>rel_image snd (rel_liftL (wssa R (nofailure_pred precond) \<^emph>\<and> nofailure_pred F) \<sqinter>
       heap_alloc_rel Ptr x e) \<le> G\<close>
-    using assms(3-4) frame_not_maximal_heap
+    using assms(3) frame_cond
     unfolding heap_alloc_rel_def precond_def maximal_heap_def
-    apply (clarsimp simp add: nofailure_pred_sepconj_conj_distrib[symmetric])
-    apply (clarsimp simp add: emp_def sepconj_conj_def wlp_def le_fun_def)
-    apply (metis maximal_perm_ex not_Some_prod_eq)
+    apply (clarsimp simp add: nofailure_pred_sepconj_conj_distrib[symmetric] emp_def wlp_def
+         sepconj_conj_def le_fun_def val_at_def plus_option_iff septract_conj_def imp_ex_conjL
+         imp_conjL)
+    apply (rename_tac ss ss' fl ls fs fls' fl')
+    apply (subgoal_tac \<open>ls = Map.empty\<close>)
+     prefer 2
+     apply fast
+    apply (elim disjE, blast)
+    apply clarsimp
+    apply (drule spec2, drule mp, assumption)
+    apply (metis fail_st.distinct(1) map_empty_disjoint(2) option.distinct(1) rtranclp.rtrancl_refl)
     done
-qed simp+
+qed (simp add: sswa_comp_ppABC_to_ppACB_distrib wssa_comp_ppABC_to_ppACB_distrib pred_times_le_iff)+
 
 
 subsection \<open> Heap Free \<close>
 
 definition heap_free_rel
-  :: \<open>'pt \<Rightarrow> ((('pt \<rightharpoonup> 'v discr \<times> 'perm::pre_perm_alg) \<times> fail_st) \<times> 's) \<Rightarrow> _ \<Rightarrow> bool\<close>
+  :: \<open>'pt \<Rightarrow> ((('pt \<rightharpoonup> 'a::pre_perm_alg) \<times> fail_st) \<times> 's) \<Rightarrow> _ \<Rightarrow> bool\<close>
   where
     \<open>heap_free_rel pt \<equiv>
       (\<lambda>(l,fl) (l',fl').
@@ -552,67 +817,88 @@ definition heap_free_rel
 
 abbreviation \<open>HeapFree pt \<equiv> \<langle> heap_free_rel pt \<rangle>\<close>
 
-
 lemma rgsat_heap_free:
   fixes pt e R p
     and \<pi> :: \<open>'perm :: pre_perm_alg\<close>
-  defines \<open>precond \<equiv> wssa R (pt \<^bold>\<mapsto>\<^bsub>\<pi>\<^esub> e \<sqinter> \<S> p)\<close>
-    and \<open>postcond \<equiv> \<L> emp \<sqinter> sswa R (\<S> p)\<close>
+  defines \<open>precond \<equiv> (\<Squnion>v. \<L> (pt \<^bold>\<mapsto> v)) \<sqinter> \<S> p\<close>
+    and \<open>postcond \<equiv> \<L> emp \<sqinter> \<S> p\<close>
   assumes
     \<open>(=) \<le> G\<close>
-    \<open>precond \<le> I\<close>
-    \<open>postcond \<le> I\<close>
+    \<open>wssa R precond \<le> I\<close>
+    \<open>sswa R postcond \<le> I\<close>
     \<open>T RGSepAtom\<close>
-    and frames_disjoint_at_pt:
-    \<open>F \<le> \<L>\<^sub>S (\<lambda>ss. heap_avoiding pt (e ss) \<pi>)\<close>
+    and frame_cond:
+    \<open>F \<sqinter> (wssa R precond \<midarrow>\<odot>\<^sub>\<and> \<top>) \<le> - \<L> (\<Squnion>v. pt \<^bold>\<mapsto>\<^sup>\<Up> v)\<close>
   shows
-    \<open>R, G, I, F, T \<turnstile>\<^sub>f { precond } HeapFree pt { postcond }\<close>
+    \<open>R, G, I, F, T \<turnstile>\<^sub>f { wssa R precond } HeapFree pt { sswa R postcond }\<close>
   using assms
 proof (intro rgsat_atom[where p=\<open>nofailure_pred precond\<close> and q=\<open>nofailure_pred postcond\<close>])
-  show \<open>nofailure_pred precond \<le> wssa R (nofailure_pred precond)\<close>
-    unfolding precond_def
-    by (clarsimp simp add: wlp_def, metis rtranclp_trans)
-  then show \<open>sswa R (nofailure_pred precond) \<le> nofailure_pred I\<close>
-    using assms(4)
-    by (meson nofailure_pred_strong_mono order.trans wlp_weaker_iff_sp_stronger)
+  let ?ra = \<open>(\<lambda>l l'. (\<exists>x. l pt = Some x \<and> l' = l(pt := None))) \<times>\<^sub>R (=)\<close>
 
-  show \<open>sswa R (nofailure_pred postcond) \<le> nofailure_pred postcond\<close>
-    unfolding postcond_def
-    by (clarsimp simp add: points_to_perm_def  emp_def sp_def heap_upd_eq_iff, metis rtranclp_trans)
-  then show \<open>sswa R (nofailure_pred postcond) \<le> nofailure_pred I\<close>
-    using assms(5) nofailure_pred_strong_mono by blast
-
-  show \<open>\<forall>f\<le>nofailure_pred F.
-          sp (heap_free_rel pt) (nofailure_pred precond \<^emph>\<and> f) \<le>
-            nofailure_pred postcond \<^emph>\<and> any_shared f\<close>
-    unfolding precond_def postcond_def heap_free_rel_def emp_def
-    apply (simp add: all_subpred_pred_times_eq_res_ppABC_to_ppACB_internalise
-        nofailure_pred_sepconj_conj_distrib[symmetric]
-        any_shared_pred_times_eq_res_ppABC_to_ppACB_distrib)
-    apply (clarsimp simp add: sp_def wlp_def points_to_perm_def sepconj_conj_def plus_option_iff)
-    apply (rename_tac lfs fl ss ls fs)
-      \<comment> \<open> Replacing \<open>x\<close> with \<open>(e ss)\<close> here causes simplifier loops. Presumably because
-            the stabilised predicate we are deriving this from can now show many \<open>e ss = e ss'\<close>
-            lemmas. \<close>
-    apply (subgoal_tac \<open>\<exists>x. ls = [pt \<mapsto> (Discr x, \<pi>)]\<close>)
-     prefer 2
-     apply force
-    apply clarsimp
-    apply (rule conjI, force)
-    apply (elim disjE)
-     apply clarsimp
-     apply (metis fun_upd_triv)
-      (* find a contradiction with the disjoint frame assm *)
-    apply (cut_tac frames_disjoint_at_pt)
-    apply (clarsimp simp add: disjoint_fun_def disjoint_option_def le_fun_def
-        heap_avoiding_def points_to_upcl_def split: if_splits)
-    apply (metis (mono_tags, lifting) fst_conv heap_upd_eq_iff rtranclp.rtrancl_refl)
+  have \<open>\<And>f. sp (heap_free_rel pt) (nofailure_pred (wssa R precond \<^emph>\<and> f)) \<le> nofailure_pred \<top>\<close>
+    unfolding heap_free_rel_def precond_def
+    apply (clarsimp simp add: sp_def wlp_def points_to_def sepconj_conj_def plus_option_iff)
+    apply (metis (full_types) fun_upd_same not_None_eq rtranclp.rtrancl_refl)
+    done
+  then have heap_free_rel_nofailure_helper:
+    \<open>\<And>f q.
+      sp (heap_free_rel pt) (nofailure_pred (wssa R precond \<^emph>\<and> f)) \<le> nofailure_pred q \<longleftrightarrow>
+        sp ?ra (wssa R precond \<^emph>\<and> f) \<le> q\<close>
+    apply (subst sp_nofailure_pred_in_out_iff)
+    apply (clarsimp simp add: heap_free_rel_def sp_def le_fun_def sepconj_conj_def)
     done
 
-  show \<open>rel_image snd (rel_liftL (nofailure_pred precond \<^emph>\<and> nofailure_pred F) \<sqinter> heap_free_rel pt) \<le> G\<close>
+  let ?frame2 = \<open>\<forall>f\<le>F. sp ?ra (wssa R precond \<^emph>\<and> f) \<le> postcond \<^emph>\<and> any_shared f\<close>
+  let ?frame1 =
+    \<open>\<forall>f\<le>nofailure_pred F.
+          sp (heap_free_rel pt) (wssa R (nofailure_pred precond) \<^emph>\<and> f) \<le>
+            nofailure_pred postcond \<^emph>\<and> any_shared f\<close>
+
+  have \<open>\<top> = (F \<sqinter> (wssa R precond \<midarrow>\<odot>\<^sub>\<and> \<top>) \<le> - \<L> (\<Squnion>v. pt \<^bold>\<mapsto>\<^sup>\<Up> v))\<close>
+    using frame_cond
+    by simp
+  also have \<open>... = ?frame2\<close>
+    apply (clarsimp simp add: sepconj_conj_def sp_def le_fun_def imp_conjL imp_ex_conjL
+        plus_option_iff septract_conj_def)
+    apply (intro iffI allI impI; clarify?)
+      (* \<Rightarrow> *)
+     apply (rename_tac ss ls fs vv)
+     apply (drule_tac spec2, drule mp, fast, drule spec, drule mp, rule disjoint_sym, assumption)
+     apply (drule mp, fast)
+     apply (subgoal_tac \<open>\<exists>v. ls = [pt \<mapsto> v]\<close>)
+      prefer 2
+      apply (simp add: precond_def wlp_def points_to_def, blast)
+     apply (simp add: precond_def postcond_def)
+     apply (clarsimp simp add: emp_def wlp_def points_to_def points_to_dom_upcl_def)
+     apply blast
+      (* \<Leftarrow> *)
+    apply (rename_tac fs ss ls vf)
+    apply (clarsimp simp add: points_to_dom_upcl_def)
+    apply (drule_tac x=\<open>(=) (fs, ss)\<close> in spec, drule mp, fast)
+    apply (subgoal_tac \<open>\<exists>v. ls = [pt \<mapsto> v]\<close>)
+     prefer 2
+     apply (simp add: precond_def wlp_def points_to_def, blast)
+    apply clarsimp
+    apply (drule_tac x=\<open>[pt \<mapsto> v] + fs\<close> in spec, drule mp, force)
+    apply (drule_tac x=\<open>[pt \<mapsto> v]\<close> in spec, drule mp)
+     apply (simp add: disjoint_sym_iff; fail)
+    apply (clarsimp simp add: postcond_def emp_def fun_eq_iff split: if_splits)
+    done
+  also have \<open>... = ?frame1\<close>
+    by (simp add: pred_times_le_iff heap_free_rel_nofailure_helper
+        all_subpred_pred_times_eq_res_ppABC_to_ppACB_internalise
+        any_shared_pred_times_eq_res_ppABC_to_ppACB_distrib
+        nofailure_pred_sepconj_conj_distrib[symmetric] wssa_comp_ppABC_to_ppACB_distrib)
+  finally show \<open>?frame1\<close>
+    unfolding postcond_def emp_def
+    by simp
+
+  show
+    \<open>rel_image snd (rel_liftL (wssa R (nofailure_pred precond) \<^emph>\<and> nofailure_pred F) \<sqinter>
+      heap_free_rel pt) \<le> G\<close>
     using assms(3)
     by (fastforce simp add: heap_free_rel_def)
-qed simp+
+qed (simp add: sswa_comp_ppABC_to_ppACB_distrib wssa_comp_ppABC_to_ppACB_distrib pred_times_le_iff)+
 
 
 end
